Introduce ByteVector arithmetic operations (#65)
Co-authored-by: Arthur Paulino <arthurleonardo.ap@gmail.com>
Co-authored-by: mpenciak <matej.penciak@gmail.com>

YatimaStdLib/ByteVector.lean
@@ -1,4 +1,5 @@
 import YatimaStdLib.ByteArray
+import Std.Data.Nat.Lemmas
 
 structure ByteVector (n : Nat) where
   data  : ByteArray
@@ -31,6 +32,28 @@ def get' (vec : ByteVector n) (i : Fin n) : UInt8 :=
 def get! (vec : ByteVector n) (i : Nat) : UInt8 :=
   vec.data.get! i
 
+def set (vec : ByteVector n) (i : Nat) (h : i < n) (u : UInt8) : ByteVector n :=
+  let data := vec.data.set ⟨i, by simp only [vec.valid, h]⟩ u
+  ⟨data, by rw [ByteArray.set_size, vec.valid]⟩
+
+def set' (vec : ByteVector n) (i : Fin n) (u : UInt8) : ByteVector n :=
+  let data := vec.data.set ⟨i, by simp only [vec.valid, i.isLt]⟩ u
+  ⟨data, by rw [ByteArray.set_size, vec.valid]⟩
+
+def set! (vec : ByteVector n) (i : Nat) (u : UInt8) : ByteVector n :=
+  let data := vec.data.set! i u
+  ⟨data, by rw [ByteArray.set!_size, vec.valid]⟩
+
+def genWith (f : Fin n → UInt8) : ByteVector n := Id.run do
+  let mut res := default
+  for h : i in [0 : n] do
+    have := Membership.mem.upper h
+    res := res.set i this (f $ Fin.mk i this)
+  return res  
+
+def ofNat (n capacity : Nat) : ByteVector capacity :=
+  ⟨n.toByteArrayLE.slice 0 capacity, ByteArray.slice_size⟩
+
 @[extern "lean_byte_vector_to_uint16"]
 opaque toUInt16 : @& ByteVector 2 → UInt16
 
@@ -39,5 +62,73 @@ opaque toUInt32 : @& ByteVector 4 → UInt32
 
 @[extern "lean_byte_vector_to_uint64"]
 opaque toUInt64 : @& ByteVector 8 → UInt64
+
+def map (v : ByteVector n) (f : UInt8 → UInt8) : ByteVector n := Id.run do
+  let mut res := default
+  for h : i in [0 : n] do
+    have := Membership.mem.upper h
+    res := res.set i this (f $ v.get i this)
+  pure res
+
+def zipWith (x y : ByteVector n) (f : UInt8 → UInt8 → UInt8) : ByteVector n := Id.run do
+  let mut res := default
+  for h : i in [0 : n] do
+    have := Membership.mem.upper h
+    res := res.set i this (f (x.get i this) (y.get i this))
+  pure res
+
+def split (x : ByteVector n) (size₁ size₂ : Nat) : ByteVector size₁ × ByteVector size₂ :=
+  let left := x.data.slice 0 size₁
+  let right := x.data.slice size₁ size₂
+  (⟨left, ByteArray.slice_size⟩, ⟨right, ByteArray.slice_size⟩)
+
+open Array in
+def append (x : ByteVector n) (y : ByteVector m) : ByteVector (n + m) := 
+  let ⟨xData, xSize⟩ := x
+  let ⟨yData, ySize⟩ := y
+  ⟨⟨xData.data ++ yData.data⟩, append_size xData.data yData.data xSize ySize⟩
+
+def shiftRight1 (x : ByteVector n) : ByteVector n := 
+  ⟨x.data.slice 1 n, ByteArray.slice_size⟩
+
+def shiftRight (x : ByteVector n) : Nat → ByteVector n
+  | 0     => x
+  | m + 1 => shiftRight (shiftRight1 x) m
+
+-- Boolean and arithmetic operations
+
+def lor (x : ByteVector n) (y : ByteVector n) : ByteVector n :=
+  x.zipWith y UInt8.lor
+
+def and (x : ByteVector n) (y : ByteVector n) : ByteVector n :=
+  x.zipWith y UInt8.land
+
+def xor (x : ByteVector n) (y : ByteVector n) : ByteVector n :=
+  x.zipWith y UInt8.xor
+
+def not (x : ByteVector n) : ByteVector n :=
+  x.map (255 - ·)
+
+def add (x y : ByteVector n) : ByteVector n := 
+  ⟨x.data + y.data |>.slice 0 n, ByteArray.slice_size⟩
+
+instance : Add (ByteVector n) where
+  add := add
+
+-- TODO: is it correct?
+instance : Sub (ByteVector n) where
+  sub x y := x + ByteVector.not y
+
+instance : HMul (ByteVector n) UInt8 (ByteVector n) where
+  hMul b u := ⟨b.data * u |>.slice 0 n, ByteArray.slice_size⟩
+
+private def naiiveMul (x y : ByteVector n) : ByteVector n :=
+  ⟨x.data * y.data |>.slice 0 n, ByteArray.slice_size⟩
+
+def karatsubaMul (x y : ByteVector n) : ByteVector n := 
+  ⟨x.data * y.data |>.slice 0 n, ByteArray.slice_size⟩
+
+instance : Mul (ByteVector n) where
+  mul := naiiveMul
 
 end ByteVector
