Benchmarks/ByteArray.lean
@@ -1,0 +1,29 @@
+import YatimaStdLib.Benchmark
+import YatimaStdLib.ByteArray
+
+open Benchmark FixedSize
+
+open RandomGen in
+instance : FixedSize Nat where
+  random n g := do
+    let mut (m, g') := RandomGen.next g.down
+    let mut answer := 0
+    for _ in [:n] do
+      (m, g') := RandomGen.next g'
+      answer := answer * 256 + (m % 256)
+    return (answer, .up g')
+
+instance : FixedSize UInt8 where
+  random _ := do
+    let n : Nat := ← random 10
+    return n.toUInt8
+
+instance : FixedSize ByteArray where
+  random size := do
+    let mut answer := default
+    for _ in [:size] do
+      answer := answer.push (← random 10)
+    return answer
+
+def main (args : List String) : IO Unit := benchmarks args (#[1024, 2048, 4096, 8192, 16384, 32768]) 
+  (fun ((b₁ : ByteArray), (b₂ : ByteArray)) => b₁ * b₂)
