YatimaStdLib/Array.lean
@@ -35,3 +35,8 @@ instance [Ord α] : Ord (Array α) where
   compare x y := compare x.data y.data
 
 def last (ar : Array α) : Array α := ar.toSubarray.popFront.toArray
+
+theorem append_size (arr₁ arr₂ : Array α) (h1 : arr₁.size = n) (h2 : arr₂.size = m) 
+    : (arr₁ ++ arr₂).size = n + m := by
+  unfold Array.size at *
+  simp [h1, h2]
