YatimaStdLib/ByteArray.lean
@@ -12,6 +12,7 @@ def asLEtoNat (b : ByteArray) : Nat :=
 def asBEtoNat (b : ByteArray) : Nat :=
   b.data.data.foldl (init := 0) fun acc bᵢ => acc.shiftLeft 8 + bᵢ.toNat
 
+/-- Returns the index of -/
 def leadingZeroBits (bytes : ByteArray) : Nat := Id.run do
   let mut c := 0
   for byte in bytes do
@@ -21,6 +22,7 @@ def leadingZeroBits (bytes : ByteArray) : Nat := Id.run do
     else c := c + zs
   return c
 
+/-- Appends `n` bytes of `0`s to a `ByteArray` -/
 def pushZeros (bytes : ByteArray) (n : Nat) : ByteArray :=
   bytes ++ ⟨.mkArray n 0⟩
 
@@ -66,7 +68,7 @@ def getBit (bs : ByteArray) (n : Nat) : Bit :=
   UInt8.getBit (getD bs idx 0) rem
 
 /--
-Shifts the byte array left by 1, preserves length (so in particular kills the
+Shifts the byte array left by 1 bit, preserves length (so in particular kills the
 first coefficient
 -/
 def shiftLeft (bs : ByteArray) : ByteArray := Id.run do
@@ -75,6 +77,9 @@ def shiftLeft (bs : ByteArray) : ByteArray := Id.run do
     answer := answer.push <|
       (getD bs idx 0 <<< 1 : UInt8) + (getD bs (idx + 1) 0 >>> 7 : UInt8)
   answer
+
+/-- Shift the `ByteArray` right by `n` bytes by prepending the `n`-length array of `0`s -/
+def shiftRight8n (bs : ByteArray) (n : Nat) := ⟨.mkArray n 0⟩ ++ bs
 
 def shiftAdd (bs : ByteArray) (b : Bit) : ByteArray :=
   let ans := shiftLeft bs
@@ -91,8 +96,7 @@ def sliceL (bs : ByteArray) (i n : Nat) : ByteArray :=
 def slice : @& ByteArray → Nat → Nat → ByteArray :=
   sliceL
 
-theorem sliceL.aux_size {n : Nat} :
-    (sliceL.aux acc n bs).size = acc.size + n := by
+theorem sliceL.aux_size : (sliceL.aux acc n bs).size = acc.size + n := by
   induction bs generalizing acc n
   · induction n <;> simp [sliceL.aux, ByteArray.size, Array.size]
   rename_i ih
@@ -103,5 +107,114 @@ theorem sliceL.aux_size {n : Nat} :
 
 theorem slice_size : (slice bytes i n).size = n := by
   simp [slice, sliceL, sliceL.aux, sliceL.aux_size, ByteArray.size]
+
+theorem set_size : (set arr i u).size = arr.size := by
+  simp [size, set]
+
+theorem set!_size : (set! arr i u).size = arr.size := by
+  simp [size, set!, Array.set!, Array.setD]
+  by_cases h : i < arr.data.size <;> simp [h]
+
+/- 
+In this section we define Arithmetic on ByteArrays viewed as natural numbers encoded in
+little-endian form
+-/
+
+section arithmetic
+
+private def uInt8OverFlowMul (u₁ u₂ : UInt8) : UInt8 × UInt8 := 
+  let u16 := u₁.toUInt16 * u₂.toUInt16
+  (u16 >>> 8 |>.toUInt8, u16.toUInt8)
+
+private def uInt8OverFlowAdd (u₁ u₂ : UInt8) : UInt8 × UInt8 :=
+  let u16 := u₁.toUInt16 + u₂.toUInt16
+  (u16 >>> 8 |>.toUInt8, u16.toUInt8)
+
+def uInt8Mul (x : ByteArray) (u : UInt8) : ByteArray := Id.run do
+  let mut carry: UInt8 := 0
+  let mut answer: ByteArray := default
+
+  for uX in x do
+    let (carry1, res') := uInt8OverFlowMul uX u
+    let (carry2, res) := uInt8OverFlowAdd carry res'
+    answer := answer.push res
+    carry := carry1 + carry2
+  
+  answer := if carry == 0 then answer else answer.push carry
+  return answer
+
+instance : HMul ByteArray UInt8 ByteArray where
+  hMul := uInt8Mul
+
+def add (x y : ByteArray) : ByteArray := Id.run do
+  let mut res := default
+  let mut cin := 0
+  let n := max x.size y.size
+
+  for i in [0 : n] do
+    let (r, o) := UInt8.sum3 cin (x.getD i 0) (y.getD i 0)
+    res := res.push r
+    cin := o
+  
+  res := if cin == 0 then res else res.push cin
+  return res
+
+instance : Add ByteArray where
+  add := add
+
+def sub (x y : ByteArray) : ByteArray := Id.run do
+  let mut res := default
+  let mut cin := 0
+  let n := max x.size y.size
+
+  for i in [0 : n] do
+    let xi := x.getD i 0
+    let yi := y.getD i 0
+    if xi < yi + cin then
+      let diff := (255 - yi - cin) + xi + 1
+      res := res.push diff
+      cin := 1 else
+      let diff := xi - yi - cin
+      res := res.push diff
+      cin := 0
+
+  return res
+
+instance : Sub ByteArray where
+  sub := sub
+
+/-- "naiive" multiplication of two ByteArrays -/
+def nmul (x y : ByteArray) : ByteArray := Id.run do
+  let mut answer: ByteArray := default
+  let mut idx := 0
+
+  for u in x do
+    let temp := y * u
+    answer := answer + temp.shiftRight8n idx
+    idx := idx + 1
+  
+  answer
+
+/-- Karatsuba multiplication of two ByteArrays -/
+partial def kmul (x y : ByteArray) : ByteArray :=
+  let n := max x.size y.size
+  if n ≤ 8 then nmul x y else 
+    let low := n / 2
+    let high := n - low
+    let xLow := x.slice 0 low
+    let yLow := y.slice 0 low
+    let xHigh := x.slice low high
+    let yHigh := y.slice low high
+    let xMid := xHigh + xLow
+    let yMid := yHigh + yLow
+    let lowMul := kmul xLow yLow
+    let highMul := kmul xHigh yHigh
+    let midMul := kmul xMid yMid - highMul - lowMul
+    highMul.shiftRight8n (2 * high) + midMul.shiftRight8n high + lowMul
+
+instance : Mul ByteArray where
+  mul := kmul
+
+end arithmetic
 
 end ByteArray
