lakefile.lean
@@ -76,5 +76,6 @@ lean_exe Tests.UInt
 
 /- Benchmarks -/
 lean_exe Benchmarks.AddChain
+lean_exe Benchmarks.ByteArray
 lean_exe Benchmarks.Matrix
 lean_exe Benchmarks.SparseMatrix
